@prefix owl: <http://www.w3.org/2002/07/owl#> .
@prefix dct: <http://purl.org/dc/terms/> .
@prefix rdfs: <http://www.w3.org/2000/01/rdf-schema#> .

@prefix ids: <http://industrialdataspace.org/2016/10/ids/core#> .
@prefix valid: <http://industrialdataspace.org/2017/01/ids/validation#> .

# Classes
# -------

ids:InfrastructureComponent a owl:Class;
    rdfs:label "InfrastructureComponent"@en ;
    rdfs:comment "The class of all infrastructure components of the IDS.";
    ids:validation [
        owl:onProperty ids:operatedBy;
        valid:constraint "@NotNull";
    ].

# Properties
# ----------

ids:title rdfs:subPropertyOf dct:title;
	a owl:DatatypeProperty;
	rdfs:label "title"@en;
	rdfs:domain ids:InfrastructureComponent;
	rdfs:range rdfs:Literal;
	rdfs:comment "Name of the BaseEntity. MUST be asserted to resources of type BaseEntity."@en.

ids:description rdfs:subPropertyOf dct:description;
	a owl:DatatypeProperty;
	rdfs:label "description"@en;
	rdfs:domain ids:InfrastructureComponent;
	rdfs:range rdfs:Literal;
	rdfs:comment "Freetext description of the BaseEntity. MAY be asserted to resources of type BaseEntity.".

ids:createdBy rdfs:subPropertyOf dct:creator;
    a owl:ObjectProperty;
    rdfs:label "createdBy"@en;
    rdfs:domain ids:InfrastructureComponent;
    rdfs:range ids:Participant;
    rdfs:comment "Participant primarily responsible for making the resource."@en.

ids:maintainedBy a owl:ObjectProperty;
    a owl:ObjectProperty;
    rdfs:label "maintainedBy"@en;
    rdfs:domain ids:InfrastructureComponent;
    rdfs:range ids:Participant;
    rdfs:comment "Participant responsible for maintaining the InfrastructureComponent."@en.

ids:operatedBy a owl:ObjectProperty;
    a owl:ObjectProperty;
    rdfs:label "operatedBy"@en;
    rdfs:domain ids:InfrastructureComponent;
    rdfs:range ids:Participant;
    rdfs:comment "Participant responsible for operating the InfrastructureComponent."@en.