@prefix owl: <http://www.w3.org/2002/07/owl#> .
@prefix dct: <http://purl.org/dc/terms/> .
@prefix rdfs: <http://www.w3.org/2000/01/rdf-schema#> .

@prefix ids: <http://industrialdataspace.org/2016/10/ids/core#> .
@prefix valid: <http://industrialdataspace.org/2017/01/ids/validation#> .

# Classes
# -------

ids:EntityWithLifecycle a owl:Class;
    rdfs:label "EntityWithLifecycle"@en ;
    rdfs:comment "The class of all individuals that are subject of a lifecycle which needs to be tracked.";
    ids:validation [
        owl:onProperty ids:lifecycleActivity;
        valid:relationType "@OneToMany";
    ].

ids:InfrastructureComponent rdfs:subClassOf ids:EntityWithLifecycle;
    a owl:Class;
    rdfs:label "InfrastructureComponent"@en ;
    rdfs:comment "The class of all infrastructure components of the IDS.";
    ids:validation [
        owl:onProperty ids:componentGenerationActivity;
        valid:constraint "@NotNull";
    ];
    ids:validation [
        owl:onProperty ids:operator;
        valid:constraint "@NotNull";
    ].

# Properties of InfrastructureComponent
# -------------------------------------

ids:title rdfs:subPropertyOf dct:title;
	a owl:DatatypeProperty;
	rdfs:label "title"@en;
	rdfs:domain ids:InfrastructureComponent;
	rdfs:range rdfs:Literal;
	rdfs:comment "Name of the BaseEntity. MUST be asserted to resources of type BaseEntity."@en.

ids:description rdfs:subPropertyOf dct:description;
	a owl:DatatypeProperty;
	rdfs:label "description"@en;
	rdfs:domain ids:InfrastructureComponent;
	rdfs:range rdfs:Literal;
	rdfs:comment "Freetext description of the BaseEntity. MAY be asserted to resources of type BaseEntity.".

ids:maintainer a owl:ObjectProperty;
    a owl:ObjectProperty;
    rdfs:label "maintainer"@en;
    rdfs:domain ids:InfrastructureComponent;
    rdfs:range ids:Participant;
    rdfs:comment "Participant responsible for maintaining the InfrastructureComponent."@en.

ids:operator a owl:ObjectProperty;
    a owl:ObjectProperty;
    rdfs:label "operator"@en;
    rdfs:domain ids:InfrastructureComponent;
    rdfs:range ids:Participant;
    rdfs:comment "Participant responsible for operating the InfrastructureComponent."@en.

# Properties of EntityWithLifecycle
# -------------------------------------

ids:generationActivity rdfs:subPropertyOf prov:wasGeneratedBy;
    a owl:ObjectProperty;
    rdfs:label "generationActivity"@en;
    rdfs:domain ids:EntityWithLifecycle;
    rdfs:range ids:CreationActivity;
    rdfs:comment "Activity that led to the generation of the InfrastructureComponent."@en.

ids:lifecycleActivity a owl:ObjectProperty;
    rdfs:label "lifecycleActivity"@en;
    rdfs:domain ids:EntityWithLifecycle;
    rdfs:range ids:Activity;
    rdfs:comment "Activity that occurs during the lifecycle of the InfrastructureComponent."@en.