@prefix owl: <http://www.w3.org/2002/07/owl#> .
@prefix rdfs: <http://www.w3.org/2000/01/rdf-schema#> .
@prefix xsd: <http://www.w3.org/2001/XMLSchema#> .
@prefix dct: <http://purl.org/dc/terms/> .
@prefix dcat: <http://www.w3.org/ns/dcat#> .
@prefix skos: <http://www.w3.org/2004/02/skos/core#> .

@prefix ids: <http://industrialdataspace.org/2016/10/ids/core#> .
@prefix valid: <http://industrialdataspace.org/2017/01/ids/validation#> .

# Classes
# -------

ids:DataAsset rdfs:subClassOf dcat:Dataset;
    a owl:Class;
    rdfs:label "DataAsset"@en;
    rdfs:comment "DataAsset on the Industrial Dataspace. May be a data offering, data that is in the state of being transfered or an aggregation of multiple other dataassets."@en;
    ids:validation [
        owl:onProperty ids:dataAssetTitle;
        valid:relationType "@OneToMany";
        valid:constraint "@javax.validation.constraints.NotNull";
    ];
    ids:validation [
        owl:onProperty ids:dataAssetDescription;
        valid:relationType "@OneToMany";
    ];
    ids:validation [
        owl:onProperty ids:contentCreator;
        valid:constraint "@javax.validation.constraints.NotNull";
    ];
    ids:validation [
        owl:onProperty ids:coversTemporal;
        valid:relationType "@OneToMany";
    ];
    ids:validation [
        owl:onProperty ids:coversSpatial;
        valid:relationType "@OneToMany";
    ];
    ids:validation [
        owl:onProperty ids:coversCategory;
        valid:relationType "@OneToMany";
    ];
    ids:validation [
        owl:onProperty ids:coversLanguage;
        valid:relationType "@OneToMany";
    ];
    ids:validation [
        owl:onProperty ids:keyword;
        valid:relationType "@OneToMany";
    ].

# Properties
# ----------

ids:dataAssetTitle rdfs:subPropertyOf dct:title;
	a owl:DatatypeProperty;
	rdfs:label "dataAssetTitle"@en;
	rdfs:domain ids:DataAsset;
	rdfs:range rdfs:Literal;
	rdfs:comment "Title of the DataAsset."@en.

ids:dataAssetDescription rdfs:subPropertyOf dct:description;
	a owl:DatatypeProperty;
	rdfs:label "dataAssetDescription"@en;
	rdfs:domain ids:DataAsset;
	rdfs:range rdfs:Literal;
	rdfs:comment "Freetext description of the DataAsset.".

ids:creationDate rdfs:subPropertyOf dct:dateSubmitted;
    a owl:DatatypeProperty;
    rdfs:label "creationDate"@en;
    rdfs:domain ids:DataAsset;
    rdfs:range xsd:dateTime;
    rdfs:comment "Date of creation of the InfrastructureComponent."@en.

ids:format rdfs:subPropertyOf dct:format;
    a owl:DatatypeProperty;
    rdfs:label "format"@en;
    rdfs:domain ids:DataAsset;
    rdfs:range xsd:string;
    rdfs:comment "The file format of the DataAsset. ids:mediaType SHOULD be used if the type of the distribution is defined by IANA."@en.

ids:mediaType rdfs:subPropertyOf dcat:mediaType;
    a owl:ObjectProperty;
    rdfs:label "mediaType"@en;
    rdfs:domain ids:DataAsset;
    rdfs:range ids:IANAMediaType;
    rdfs:comment "The media type of the DataAsset, as defined by IANA."@en.

ids:version rdfs:subPropertyOf dct:hasVersion;
    a owl:DatatypeProperty;
    rdfs:label "version"@en;
    rdfs:domain ids:DataAsset;
    rdfs:range xsd:string;
    rdfs:comment "Version identifier of the InfrastructureComponent."@en.

ids:contentCreator
    a owl:ObjectProperty;
    rdfs:label "contentCreator"@en;
    rdfs:domain ids:DataAsset;
    rdfs:range xsd:anyURI;
    rdfs:comment "Participant responsible for creating the content of the DataAsset."@en.

ids:conformsToStandard
    a owl:DatatypeProperty;
    rdfs:label "conformsTo"@en;
    rdfs:domain ids:DataAsset;
    rdfs:range xsd:anyURI;
    rdfs:comment "The standard the DataAsset conforms to."@en.

ids:licenseDocument rdfs:subPropertyOf dct:license;
    a owl:ObjectProperty;
    rdfs:label "licenseDocument"@en;
    rdfs:domain ids:DataAsset;
    rdfs:range ids:LicenseDocument;
    rdfs:comment "License of the DataAsset. Refers to common standard licenses used in the IDS."@en.

ids:licenseReference rdfs:subPropertyOf dct:license;
    a owl:ObjectProperty;
    rdfs:label "licenseReference"@en;
    rdfs:domain ids:DataAsset;
    rdfs:range xsd:anyURI;
    rdfs:comment "References a license document that is publicly available on the Web."@en.

ids:coversIndustry a owl:ObjectProperty;
    rdfs:label "coversIndustry"@en;
    rdfs:domain ids:DataAsset;
    rdfs:range ids:ISICIndustry;
    rdfs:comment "Industry branch covered by the DataAsset."@en.

ids:coversTemporal rdfs:subPropertyOf dct:temporal;
    rdfs:label "coversTemporal"@en;
    rdfs:domain ids:DataAsset;
    rdfs:range ids:TemporalEntity;
    rdfs:comment "Temporal period or instance covered by the DataAsset."@en.

ids:coversSpatial rdfs:subPropertyOf dct:spatial;
    rdfs:label "coversSpatial"@en;
    rdfs:domain ids:DataAsset;
    rdfs:range ids:SpatialEntity;
    rdfs:comment "Spatial location covered by the DataAsset."@en.

ids:conformsToStructure a owl:ObjectProperty;
    rdfs:label "conformsToStructure"@en;
    rdfs:domain ids:DataAsset;
    rdfs:range xsd:anyURI;
    rdfs:comment "Links to a document that contains additional information like class and type descriptions or integrity constraints describing the DataAssets structure."@en.

ids:transformationRule a owl:ObjectProperty;
    rdfs:label "transformationRule"@en;
    rdfs:domain ids:DataAsset;
    rdfs:range xsd:anyURI;
    rdfs:comment "Links to a document that contains rules or algorithms to transform the DataAsset into another representation while retaining the information content."@en.

ids:coversCategory rdfs:subPropertyOf dcat:theme;
    rdfs:label "coversCategory"@en;
    rdfs:domain ids:DataAsset;
    rdfs:range xsd:anyURI;
    rdfs:comment "Links to a taxonomy categorizing content-related coverage of the DataAsset."@en.

ids:keyword rdfs:subPropertyOf dcat:theme;
    rdfs:label "keyword"@en;
    rdfs:domain ids:DataAsset;
    rdfs:range xsd:anyURI;
    rdfs:comment "Links to an item in a flat list of controlled keywords that describe content-related coverage of the DataAsset."@en.

ids:volume a owl:DatatypeProperty;
    rdfs:label "volume"@en;
    rdfs:domain ids:DataAsset;
    rdfs:range xsd:long;
    rdfs:comment "The total uncompressed size of the dataset in MB."@en.

ids:coversLanguage rdfs:subPropertyOf dct:language;
    rdfs:label "coversLanguage"@en;
    rdfs:domain ids:DataAsset;
    rdfs:range ids:Language;
    rdfs:comment "States the language that is used in the DataAsset."@en.