@prefix owl: <http://www.w3.org/2002/07/owl#> .
@prefix rdfs: <http://www.w3.org/2000/01/rdf-schema#> .
@prefix foaf: <http://xmlns.com/foaf/0.1/> .
@prefix org: <http://www.w3.org/ns/org#> .
@prefix xsd: <http://www.w3.org/2001/XMLSchema#> .

@prefix ids: <http://industrialdataspace.org/2016/10/ids/core#> .
@prefix valid: <http://industrialdataspace.org/2017/01/ids/validation#> .

# Classes
# -------

ids:Participant rdfs:subClassOf ids:EntityWithLifecycle;
    a owl:Class;
    rdfs:subClassOf org:Organization;
	rdfs:label "Participant"@en;
	rdfs:comment "An organization being part of the Industrial Data Space"@en.

ids:Site a owl:Class;
    rdfs:subclassOf org:Site;
    rdfs:label "Site"@en;
	rdfs:comment "An office or other premise at which the organization is located"@en.

# Properties for describing a Participant
# ---------------------------------------

ids:primarySite rdfs:subPropertyOf org:hasPrimarySite;
    a owl:ObjectProperty;
    rdfs:label "primarySite"@en;
    rdfs:domain ids:Participant;
    rdfs:range ids:Site;
    rdfs:comment "Indicates a primary site for the Organization, this is the default means by which an Organization can be contacted and is not necessarily the formal headquarters."@en.

ids:email rdfs:subPropertyOf foaf:mbox;
    a owl:DatatypeProperty;
    rdfs:label "email"@en;
    rdfs:domain ids:Participant;
    rdfs:range xsd:string;
    rdfs:comment "Email address for contacting the participant on a general level."@en.

ids:homepage rdfs:subPropertyOf foaf:homepage;
    a owl:DatatypeProperty;
    rdfs:label "homepage"@en;
    rdfs:domain ids:Participant;
    rdfs:range xsd:anyURI;
    rdfs:comment "General official homepage of the participant."@en.

# Properties for describing a Site
# --------------------------------

ids:siteAddress rdfs:subPropertyOf org:siteAddress;
    a owl:ObjectProperty;
    rdfs:domain ids:Site;
    rdfs:range xsd:string;
    rdfs:label "siteAddress"@en;
    rdfs:comment "Indicates an address for the site."@en.