@prefix owl: <http://www.w3.org/2002/07/owl#> .
@prefix dct: <http://purl.org/dc/terms/> .
@prefix rdfs: <http://www.w3.org/2000/01/rdf-schema#> .
@prefix prov: <http://www.w3.org/ns/prov#> .
@prefix rdf: <http://www.w3.org/1999/02/22-rdf-syntax-ns#> .

@prefix ids: <http://industrialdataspace.org/2016/10/ids/core#> .
@prefix valid: <http://industrialdataspace.org/2017/01/ids/validation#> .
@prefix idoc: <http://industrialdataspace.org/2017/01/ids/documentation#> .
@prefix trns: <http://industrialdataspace.org/2017/01/ids/transformation#> .


# Description of this ontology
# ----------------------------

ids: a owl:Ontology;
    dct:title "The Industrial Dataspace Information Model"@en;
    rdfs:comment "This ontology defines classes and properties for describing participants, infrastructure, data and services of the Industrial Dataspace.";
    dct:creator "Christian Mader" ;
    dct:creator "Jaroslav Pullmann" ;
    dct:creator "Niklas Petersen" ;
    dct:creator "Christoph Lange-Bever" ;
    dct:creator "Steffen Lohmann" ;
    dct:publisher "Fraunhofer IAIS/EIS";
    dct:publisher "Fraunhofer FIT";
    dct:date "2017-06-20";
    owl:versionInfo "0.9.0".

# Classes
# -------

ids:EntityWithLifecycle a owl:Class;
    trns:isAbstract true;
    rdfs:label "EntityWithLifecycle"@en ;
    rdfs:comment "The class of all individuals that are subject of a lifecycle which needs to be tracked.";
    ids:validation [
        owl:onProperty ids:lifecycleActivity;
        valid:relationType "@OneToMany";
    ];
    ids:validation [
        owl:onProperty ids:entityName;
        valid:relationType "@OneToMany";
        valid:constraint "@NotNull";
    ];
    ids:validation [
        owl:onProperty ids:entityDescription;
        valid:relationType "@OneToMany";
    ].

ids:InfrastructureComponent rdfs:subClassOf ids:EntityWithLifecycle;
    a owl:Class;
    trns:isAbstract true;
    rdfs:label "InfrastructureComponent"@en ;
    rdfs:comment "The class of all infrastructure components of the IDS.";
    ids:validation [
        owl:onProperty ids:operator;
        valid:constraint "@NotNull";
    ].

# Properties of InfrastructureComponent
# -------------------------------------

ids:maintainer a owl:ObjectProperty;
    rdfs:label "maintainer"@en;
    rdfs:domain ids:InfrastructureComponent;
    rdfs:range ids:Participant;
    trns:refByURI true;
    rdfs:comment "Participant responsible for maintaining the InfrastructureComponent."@en.

ids:operator a owl:ObjectProperty;
    rdfs:label "operator"@en;
    rdfs:domain ids:InfrastructureComponent;
    rdfs:range ids:Participant;
    trns:refByURI true;
    rdfs:comment "Participant responsible for operating the InfrastructureComponent."@en.

ids:owner a owl:ObjectProperty;
    rdfs:label "owner"@en;
    rdfs:domain ids:InfrastructureComponent;
    rdfs:range ids:Participant;
    trns:refByURI true;
    rdfs:comment "Participant owning the InfrastructureComponent."@en.

ids:physicalLocation a owl:ObjectProperty;
    rdfs:label "physicalLocation"@en;
    rdfs:domain ids:InfrastructureComponent;
    rdfs:range ids:Location;
    rdfs:comment "The location where the Connector is physically deployed."@en.

# Properties of EntityWithLifecycle
# -------------------------------------

ids:entityName rdfs:subPropertyOf dct:title;
	a owl:DatatypeProperty;
	rdfs:domain ids:EntityWithLifecycle;
	rdfs:range rdf:PlainLiteral;
    rdfs:label "entityName"@en;
    idoc:labelPluralForm "entityNames"@en;
	rdfs:comment "Name of the EntityWithLifecycle."@en.

ids:entityDescription rdfs:subPropertyOf dct:description;
	a owl:DatatypeProperty;
	rdfs:domain ids:EntityWithLifecycle;
	rdfs:range rdf:PlainLiteral;
	rdfs:label "entityDescription"@en;
	idoc:labelPluralForm "entityDescriptions"@en;
	rdfs:comment "Freetext description of the EntityWithLifecycle.".

ids:generationActivity rdfs:subPropertyOf prov:wasGeneratedBy;
    a owl:ObjectProperty;
    rdfs:label "generationActivity"@en;
    rdfs:domain ids:InfrastructureComponent;
    rdfs:range ids:CreationActivity;
    rdfs:comment "Activity that led to the generation of the InfrastructureComponent."@en.

ids:lifecycleActivity a owl:ObjectProperty;
    rdfs:label "lifecycleActivity"@en;
    idoc:labelPluralForm "lifecycleActivities"@en;
    rdfs:domain ids:EntityWithLifecycle;
    rdfs:range ids:Activity;
    rdfs:comment "Activity that occurs during the lifecycle of the InfrastructureComponent."@en.